add permissions to Array, ArrayPtr

ulib/experimental/Steel.Array.fst
@@ -79,105 +79,113 @@ let vnil
 
 let vcons_rewrite
   (#t: Type)
+  (p: perm)
   (n: Ghost.erased nat)
   (r: Ghost.erased (ref t))
   (v: vprop)
   (sq: squash (t_of v == Seq.lseq t n))
-  (xy: t_of (vptr r `star` v))
+  (xy: t_of (vptrp r p `star` v))
 : GTot (Seq.lseq t (n + 1))
 = Seq.cons (fst xy) (snd xy)
 
 let vcons
   (#t: Type)
+  (p: perm)
   (n: Ghost.erased nat)
   (r: Ghost.erased (ref t))
   (v: vprop)
 : Pure vprop
   (requires (t_of v == Seq.lseq t n))
   (ensures (fun v' -> t_of v' == Seq.lseq t (n + 1)))
-= vrewrite (vptr r `star` v) (vcons_rewrite n r v ())
+= vrewrite (vptrp r p `star` v) (vcons_rewrite p n r v ())
 
 let rec varray1
   (#t: Type0)
   (a: array2 t)
+  (p: perm)
 : Pure vprop
   (requires True)
   (ensures (fun v -> t_of v == Seq.lseq t (Seq.length a)))
   (decreases (Seq.length a))
 = if Seq.length a = 0
   then vnil t
-  else vcons (Seq.length a - 1) (Seq.index a 0) (varray1 (Seq.slice a 1 (Seq.length a)))
+  else vcons p (Seq.length a - 1) (Seq.index a 0) (varray1 (Seq.slice a 1 (Seq.length a)) p)
 
 [@@ __steel_reduce__]
 unfold
 let sel_varray1 (#a:Type) (#p:vprop) (r:array2 a)
-  (h:rmem p{FStar.Tactics.with_tactic selector_tactic (can_be_split p (varray1 r) /\ True)})
+  (q: perm)
+  (h:rmem p{FStar.Tactics.with_tactic selector_tactic (can_be_split p (varray1 r q) /\ True)})
 : GTot (Seq.lseq a (Seq.length r))
-= let x : t_of (varray1 r) = h (varray1 r) in
+= let x : t_of (varray1 r q) = h (varray1 r q) in
   x
 
 let sel_varray2
   (#a: Type0)
   (r: array2 a)
-: Tot (selector (Seq.lseq a (Seq.length r)) (hp_of (varray1 r)))
-= fun h -> sel_of (varray1 r) h
+  (p: perm)
+: Tot (selector (Seq.lseq a (Seq.length r)) (hp_of (varray1 r p)))
+= fun h -> sel_of (varray1 r p) h
 
 [@@ __steel_reduce__]
-let varray2' (#a: Type0) (r: array2 a) : vprop' =
-  {hp = hp_of (varray1 r);
+let varray2' (#a: Type0) (r: array2 a) (p: perm) : vprop' =
+  {hp = hp_of (varray1 r p);
    t = Seq.lseq a (Seq.length r);
-   sel = sel_varray2 r}
+   sel = sel_varray2 r p}
 
 [@@ __steel_reduce__]
-let varray2 r = VUnit (varray2' r)
+let varray2 r p = VUnit (varray2' r p)
 
 let varray9
   (#t: Type0)
   (a: array t)
+  (p: perm)
 : Tot vprop
-= varray2 (Seq.slice a.base (U32.v a.from) (U32.v a.to))
+= varray2 (Seq.slice a.base (U32.v a.from) (U32.v a.to)) p
 
-let is_array #a r = hp_of (varray9 r)
+let is_array #a r p = hp_of (varray9 r p)
 
-let array_sel #a r = fun h -> sel_of (varray9 r) h
+let array_sel #a r p = fun h -> sel_of (varray9 r p) h
 
 let intro_varray
   (#opened: _)
   (#t: Type)
+  (p: perm)
   (q: array2 t)
   (r: array t)
 : SteelGhost unit opened
-    (varray2 q)
-    (fun _ -> varray r)
+    (varray2 q p)
+    (fun _ -> varrayp r p)
     (fun _ -> Ghost.reveal q `Seq.equal` Seq.slice r.base (U32.v r.from) (U32.v r.to))
     (fun h _ h' ->
-      (h (varray2 q) <: Seq.seq t) == h' (varray r)
+      (h (varray2 q p) <: Seq.seq t) == h' (varrayp r p)
     )
 =
   change_slprop_rel
-    (varray2 q)
-    (varray r)
-    (fun (x: t_of (varray2 q)) (y: t_of (varray r)) -> (x <: Seq.seq t) == y)
+    (varray2 q p)
+    (varrayp r p)
+    (fun (x: t_of (varray2 q p)) (y: t_of (varrayp r p)) -> (x <: Seq.seq t) == y)
     (fun _ -> ())
 
 let elim_varray
   (#opened: _)
   (#t: Type)
   (r: array t)
+  (p: perm)
 : SteelGhost (array2 t) opened
-    (varray r)
-    (fun q -> varray2 q)
+    (varrayp r p)
+    (fun q -> varray2 q p)
     (fun _ -> True)
     (fun h q h' ->
       Ghost.reveal q == Seq.slice r.base (U32.v r.from) (U32.v r.to) /\
-      (h (varray r) <: Seq.seq t) == h' (varray2 q)
+      (h (varrayp r p) <: Seq.seq t) == h' (varray2 q p)
     )
 =
   let q : array2 t = (Seq.slice r.base (U32.v r.from) (U32.v r.to)) in
   change_slprop_rel
-    (varray r)
-    (varray2 q)
-    (fun (y: t_of (varray r)) (x: t_of (varray2 q)) -> (x <: Seq.seq t) == y)
+    (varrayp r p)
+    (varray2 q p)
+    (fun (y: t_of (varray r)) (x: t_of (varray2 q p)) -> (x <: Seq.seq t) == y)
     (fun _ -> ());
   q
 
@@ -185,44 +193,47 @@ let intro_varray2
   (#opened: _)
   (#t: Type)
   (q: array2 t)
+  (p: perm)
 : SteelGhost unit opened
-    (varray1 q)
-    (fun _ -> varray2 q)
+    (varray1 q p)
+    (fun _ -> varray2 q p)
     (fun _ -> True)
     (fun h _ h' ->
-      (h' (varray2 q) <: Seq.seq t) == sel_varray1 q h 
+      (h' (varray2 q p) <: Seq.seq t) == sel_varray1 q p h
     )
 =
   change_slprop_rel
-    (varray1 q)
-    (varray2 q)
-    (fun (x: t_of (varray1 q)) (y: t_of (varray2 q)) -> (x <: Seq.seq t) == y)
+    (varray1 q p)
+    (varray2 q p)
+    (fun (x: t_of (varray1 q p)) (y: t_of (varray2 q p)) -> (x <: Seq.seq t) == y)
     (fun _ -> ())
 
 let elim_varray2
   (#opened: _)
   (#t: Type)
   (r: array2 t)
+  (p: perm)
 : SteelGhost unit opened
-    (varray2 r)
-    (fun _ -> varray1 r)
+    (varray2 r p)
+    (fun _ -> varray1 r p)
     (fun _ -> True)
     (fun h _ h' ->
-      (h (varray2 r) <: Seq.seq t) == sel_varray1 r h'
+      (h (varray2 r p) <: Seq.seq t) == sel_varray1 r p h'
     )
 =
   change_slprop_rel
-    (varray2 r)
-    (varray1 r)
-    (fun (y: t_of (varray2 r)) (x: t_of (varray1 r)) -> (x <: Seq.seq t) == y)
+    (varray2 r p)
+    (varray1 r p)
+    (fun (y: t_of (varray2 r p)) (x: t_of (varray1 r p)) -> (x <: Seq.seq t) == y)
     (fun _ -> ())
 
 let intro_vnil1
   (#opened: _)
   (t: Type)
+  (p: perm)
 : SteelGhost (array2 t) opened
     emp
-    (fun r -> varray1 r)
+    (fun r -> varray1 r p)
     (fun _ -> True)
     (fun _ r _ -> Seq.length r == 0)
 =
@@ -230,70 +241,73 @@ let intro_vnil1
   let r : array2 t = Seq.empty in
   change_slprop
     (vrewrite emp (vnil_rewrite t))
-    (varray1 r)
+    (varray1 r p)
     (Ghost.hide (Seq.empty #t <: t_of (vrewrite emp (vnil_rewrite t))))
-    (Ghost.hide (Seq.empty #t <: t_of (varray1 r)))
+    (Ghost.hide (Seq.empty #t <: t_of (varray1 r p)))
     (fun _ -> ());
   r
 
 let intro_vnil
   (#opened: _)
   (t: Type)
+  (p: perm)
 : SteelGhost (array2 t) opened
     emp
-    (fun r -> varray2 r)
+    (fun r -> varray2 r p)
     (fun _ -> True)
     (fun _ r h' ->
       Ghost.reveal r == Seq.empty /\
-      h' (varray2 r) == Seq.empty
+      h' (varray2 r p) == Seq.empty
     )
 =
   seq_facts ();
-  let res = intro_vnil1 t in
-  intro_varray2 res;
+  let res = intro_vnil1 t p in
+  intro_varray2 res _;
   res
 
 let intro_vcons1
   (#opened: _)
   (#t: Type)
+  (p: perm)
   (r: Ghost.erased (ref t))
   (a: array2 t)
 : SteelGhost (array2 t) opened
-    (vptr r `star` varray1 a)
-    (fun a' -> varray1 a')
+    (vptrp r p `star` varray1 a p)
+    (fun a' -> varray1 a' p)
     (fun _ -> fits32 (Seq.length a + 1))
     (fun h a' h' ->
       Ghost.reveal a' == Seq.cons (Ghost.reveal r) a /\
-      (sel_varray1 a' h' <: Seq.seq t) ==
-        Seq.cons (h (vptr r)) (sel_varray1 a h)
+      (sel_varray1 a' p h' <: Seq.seq t) ==
+        Seq.cons (h (vptrp r p)) (sel_varray1 a p h)
     )
 =
   seq_facts ();
-  reveal_star (vptr r) (varray1 a); // FIXME: WHY WHY WHY?
-  intro_vrewrite (vptr r `star` varray1 a) (vcons_rewrite (Seq.length a) r (varray1 a) ());
+  reveal_star (vptrp r p) (varray1 a p); // FIXME: WHY WHY WHY?
+  intro_vrewrite (vptrp r p `star` varray1 a p) (vcons_rewrite p (Seq.length a) r (varray1 a p) ());
   let a' : array2 t = Seq.cons (Ghost.reveal r) a in
   change_equal_slprop
-    (vrewrite (vptr r `star` varray1 a) (vcons_rewrite (Seq.length a) r (varray1 a) ()))
-    (varray1 a');
+    (vrewrite (vptrp r p `star` varray1 a p) (vcons_rewrite p (Seq.length a) r (varray1 a p) ()))
+    (varray1 a' p);
   a'
 
 let intro_vcons
   (#opened: _)
   (#t: Type)
+  (p: perm)
   (r: Ghost.erased (ref t))
   (a: array2 t)
 : SteelGhost (array2 t) opened
-    (vptr r `star` varray2 a)
-    (fun a' -> varray2 a')
+    (vptrp r p `star` varray2 a p)
+    (fun a' -> varray2 a' p)
     (fun _ -> fits32 (Seq.length a + 1))
     (fun h a' h' ->
       Ghost.reveal a' == Seq.cons (Ghost.reveal r) a /\
-      h' (varray2 a') ==
-        Seq.cons (h (vptr r)) (h (varray2 a))
+      h' (varray2 a' p) ==
+        Seq.cons (h (vptrp r p)) (h (varray2 a p))
     )
-= elim_varray2 a;
-  let res = intro_vcons1 r a in
-  intro_varray2 res;
+= elim_varray2 a p;
+  let res = intro_vcons1 p r a in
+  intro_varray2 res p;
   res
 
 #set-options "--ide_id_info_off" 
@@ -305,15 +319,16 @@ let elim_vcons1
   (#opened: _)
   (#t: Type)
   (a: array2 t)
+  (p: perm)
 : SteelGhost (Ghost.erased (ref t) & array2 t) opened
-    (varray1 a)
-    (fun res -> vptr (pfst res) `star` varray1 (psnd res))
+    (varray1 a p)
+    (fun res -> vptrp (pfst res) p `star` varray1 (psnd res) p)
     (fun _ -> Seq.length a > 0)
     (fun h res h' ->
       Seq.length a > 0 /\
-      begin let s = sel_varray1 a h in
-      h' (vptr (pfst res)) == Seq.head s /\
-      Seq.tail s == sel_varray1 (psnd res) h' /\
+      begin let s = sel_varray1 a p h in
+      h' (vptrp (pfst res) p) == Seq.head s /\
+      Seq.tail s == sel_varray1 (psnd res) p h' /\
       Ghost.reveal a == Seq.cons (Ghost.reveal (pfst res)) (psnd res)
       end
     )
@@ -323,15 +338,15 @@ let elim_vcons1
   let r : Ghost.erased (ref t) = (Seq.head a0) in
   let q : array2 t = Seq.tail a0 in
   change_equal_slprop
-    (varray1 a)
-    (vrewrite (vptr (r) `star` varray1 (q)) (vcons_rewrite (Seq.length (q)) (r) (varray1 (q)) ()));
-  elim_vrewrite (vptr (r) `star` varray1 (q)) (vcons_rewrite (Seq.length (q)) (r) (varray1 (q)) ());
-  reveal_star (vptr (r)) (varray1 (q));
+    (varray1 a p)
+    (vrewrite (vptrp (r) p `star` varray1 (q) p) (vcons_rewrite p (Seq.length (q)) (r) (varray1 (q) p) ()));
+  elim_vrewrite (vptrp (r) p `star` varray1 (q) p) (vcons_rewrite p (Seq.length (q)) (r) (varray1 (q) p) ());
+  reveal_star (vptrp (r) p) (varray1 (q) p);
   let res : (Ghost.erased (ref t) & array2 t) = (r, q) in
   change_equal_slprop
-    (vptr (r) `star` varray1 (q))
-    (vptr (pfst res) `star` varray1 (psnd res));
-  reveal_star (vptr (pfst res)) (varray1 (psnd res));
+    (vptrp (r) p `star` varray1 (q) p)
+    (vptrp (pfst res) p `star` varray1 (psnd res) p);
+  reveal_star (vptrp (pfst res) p) (varray1 (psnd res) p);
   res
 
 #pop-options
@@ -340,36 +355,38 @@ let elim_vcons
   (#opened: _)
   (#t: Type)
   (a: array2 t)
+  (p: perm)
 : SteelGhost (Ghost.erased (ref t) & array2 t) opened
-    (varray2 a)
-    (fun res -> vptr (pfst res) `star` varray2 (psnd res))
+    (varray2 a p)
+    (fun res -> vptrp (pfst res) p `star` varray2 (psnd res) p)
     (fun _ -> Seq.length a > 0)
     (fun h res h' ->
       Seq.length a > 0 /\
-      begin let s = h (varray2 a) in
-      s == Seq.cons (h' (vptr (pfst res))) (h' (varray2 (psnd res))) /\
+      begin let s = h (varray2 a p) in
+      s == Seq.cons (h' (vptrp (pfst res) p)) (h' (varray2 (psnd res) p)) /\
       Ghost.reveal a == Seq.cons (Ghost.reveal (pfst res)) (psnd res)
       end
     )
 =
-  elim_varray2 a;
-  let res = elim_vcons1 a in
-  intro_varray2 (psnd res);
+  elim_varray2 a p;
+  let res = elim_vcons1 a p in
+  intro_varray2 (psnd res) p;
   res
 
 let elim_nil
   (#opened: _)
   (#t: Type)
   (a: array2 t)
+  (p: perm)
 : SteelGhost unit opened
-    (varray2 a)
+    (varray2 a p)
     (fun _ -> emp)
     (fun _ -> Seq.length a == 0)
     (fun _ _ _ -> True)
 =
-  elim_varray2 a; 
+  elim_varray2 a p; 
   change_equal_slprop
-    (varray1 a)
+    (varray1 a p)
     (vrewrite emp (vnil_rewrite t));
   elim_vrewrite emp (vnil_rewrite t)
 
@@ -403,12 +420,13 @@ let rec vappend
   (#opened: _)
   (#t: Type)
   (a1 a2: array2 t)
+  (p: perm)
 : SteelGhost (array2 t) opened
-    (varray2 a1 `star` varray2 a2)
-    (fun r -> varray2 r)
+    (varray2 a1 p `star` varray2 a2 p)
+    (fun r -> varray2 r p)
     (fun _ -> fits32 (Seq.length a1 + Seq.length a2))
     (fun h r h' ->
-      h' (varray2 r) == Seq.append (h (varray2 a1)) (h (varray2 a2)) /\
+      h' (varray2 r p) == Seq.append (h (varray2 a1 p)) (h (varray2 a2 p)) /\
       Ghost.reveal r == Seq.append a1 a2
     )
     (decreases (Seq.length a1))
@@ -416,13 +434,13 @@ let rec vappend
   seq_facts ();
   if Seq.length a1 = 0
   then begin
-    elim_nil a1;
+    elim_nil a1 p;
     a2
   end else begin
-    let hd_tl = elim_vcons a1 in
-    reveal_star_3 (vptr (pfst hd_tl)) (varray2 (psnd hd_tl)) (varray2 a2); // FIXME: WHY WHY WHY?
-    let tl' = vappend (psnd hd_tl) a2 in
-    let res = intro_vcons (pfst hd_tl) tl' in
+    let hd_tl = elim_vcons a1 p in
+    reveal_star_3 (vptrp (pfst hd_tl) p) (varray2 (psnd hd_tl) p) (varray2 a2 p); // FIXME: WHY WHY WHY?
+    let tl' = vappend (psnd hd_tl) a2 p in
+    let res = intro_vcons p (pfst hd_tl) tl' in
     res
   end
 
@@ -452,52 +470,53 @@ let slice_cons_right
 let rec vsplit0
   (#opened: _)
   (#t: Type)
+  (p: perm)
   (a: array2 t)
   (i: U32.t)
 : SteelGhost (array2 t & array2 t) opened
-    (varray2 a)
-    (fun res -> varray2 (pfst res) `star` varray2 (psnd res))
+    (varray2 a p)
+    (fun res -> varray2 (pfst res) p `star` varray2 (psnd res) p)
     (fun _ -> U32.v i <= Seq.length a)
     (fun h res h' ->
-      let s = h (varray2 a) in
+      let s = h (varray2 a p) in
       U32.v i <= Seq.length a /\
       pfst res `Seq.equal` Seq.slice a 0 (U32.v i) /\
       psnd res `Seq.equal` Seq.slice a (U32.v i) (Seq.length a) /\
-      h' (varray2 (pfst res)) == Seq.slice s 0 (U32.v i) /\
-      h' (varray2 (psnd res)) `Seq.equal` Seq.slice s (U32.v i) (Seq.length a)
+      h' (varray2 (pfst res) p) == Seq.slice s 0 (U32.v i) /\
+      h' (varray2 (psnd res) p) `Seq.equal` Seq.slice s (U32.v i) (Seq.length a)
     )
     (decreases (U32.v i))
 =
   seq_facts ();
-  let g0 = gget (varray2 a) in
+  let g0 = gget (varray2 a p) in
   if i = 0ul
   then begin
-    let n = intro_vnil t in
-    reveal_star (varray2 n) (varray2 a);
+    let n = intro_vnil t p in
+    reveal_star (varray2 n p) (varray2 a p);
     let res = (n, a) in
     change_equal_slprop
-      (varray2 n `star` varray2 a)
-      (varray2 (pfst res) `star` varray2 (psnd res));
-    reveal_star (varray2 (pfst res)) (varray2 (psnd res));
+      (varray2 n p `star` varray2 a p)
+      (varray2 (pfst res) p `star` varray2 (psnd res) p);
+    reveal_star (varray2 (pfst res) p) (varray2 (psnd res) p);
     res
   end else begin
-    let hd_tl : (Ghost.erased (ref t) & array2 t) = elim_vcons a in
-    reveal_star (vptr (pfst hd_tl)) (varray2 (psnd hd_tl));
+    let hd_tl : (Ghost.erased (ref t) & array2 t) = elim_vcons a p in
+    reveal_star (vptrp (pfst hd_tl) p) (varray2 (psnd hd_tl) p);
     let j = i `U32.sub` 1ul in
     assert (U32.v j == U32.v i - 1);
-    let g2_hd = gget (vptr (pfst hd_tl)) in
-    let g2_tl = gget (varray2 (psnd hd_tl)) in
+    let g2_hd = gget (vptrp (pfst hd_tl) p) in
+    let g2_tl = gget (varray2 (psnd hd_tl) p) in
     slice_cons_left (Ghost.reveal g2_hd) (Ghost.reveal g2_tl) (U32.v i);
     slice_cons_right (Ghost.reveal g2_hd) (Ghost.reveal g2_tl) (U32.v i);
-    let sl_sr = vsplit0 (psnd hd_tl) j in
-    reveal_star_3 (vptr (pfst hd_tl)) (varray2 (pfst sl_sr)) (varray2 (psnd sl_sr)); // FIXME: WHY WHY WHY?
-    let sl = intro_vcons (pfst hd_tl) (pfst sl_sr) in
-    reveal_star (varray2 sl) (varray2 (psnd sl_sr));
+    let sl_sr = vsplit0 p (psnd hd_tl) j in
+    reveal_star_3 (vptrp (pfst hd_tl) p) (varray2 (pfst sl_sr) p) (varray2 (psnd sl_sr) p); // FIXME: WHY WHY WHY?
+    let sl = intro_vcons p (pfst hd_tl) (pfst sl_sr) in
+    reveal_star (varray2 sl p) (varray2 (psnd sl_sr) p);
     let res = (sl, psnd sl_sr) in
     change_equal_slprop
-      (varray2 sl `star` varray2 (psnd sl_sr))
-      (varray2 (pfst res) `star` varray2 (psnd res));
-    reveal_star (varray2 (pfst res)) (varray2 (psnd res));
+      (varray2 sl p `star` varray2 (psnd sl_sr) p)
+      (varray2 (pfst res) p `star` varray2 (psnd res) p);
+    reveal_star (varray2 (pfst res) p) (varray2 (psnd res) p);
     res
   end
 
@@ -506,30 +525,31 @@ let rec vsplit0
 val vsplit
   (#opened: _)
   (#t: Type)
+  (p: perm)
   (a: array2 t)
   (i: U32.t)
 : SteelGhost (array2 t & array2 t) opened
-    (varray2 a)
-    (fun res -> varray2 (pfst res) `star` varray2 (psnd res))
+    (varray2 a p)
+    (fun res -> varray2 (pfst res) p `star` varray2 (psnd res) p)
     (fun _ -> U32.v i <= Seq.length a)
     (fun h res h' ->
-      let s = h (varray2 a) in
+      let s = h (varray2 a p) in
       U32.v i <= Seq.length a /\
       pfst res `Seq.equal` Seq.slice a 0 (U32.v i) /\
       psnd res `Seq.equal` Seq.slice a (U32.v i) (Seq.length a) /\
       (a <: Seq.seq (ref t)) == Seq.append (pfst res) (psnd res) /\
-      h' (varray2 (pfst res)) == Seq.slice s 0 (U32.v i) /\
-      h' (varray2 (psnd res)) `Seq.equal` Seq.slice s (U32.v i) (Seq.length a) /\
-      s == Seq.append (h' (varray2 (pfst res))) (h' (varray2 (psnd res)))
+      h' (varray2 (pfst res) p) == Seq.slice s 0 (U32.v i) /\
+      h' (varray2 (psnd res) p) `Seq.equal` Seq.slice s (U32.v i) (Seq.length a) /\
+      s == Seq.append (h' (varray2 (pfst res) p)) (h' (varray2 (psnd res) p))
     )
 
 let vsplit
-  #_ #t a i
+  #_ #t p a i
 =
-  let g = gget (varray2 a) in
+  let g = gget (varray2 a p) in
   Seq.lemma_split a (U32.v i);
   Seq.lemma_split #t (Ghost.reveal g) (U32.v i);
-  vsplit0 a i
+  vsplit0 p a i
 
 [@@erasable]
 noeq
@@ -546,32 +566,33 @@ type ith_t
 let unpack_ith
   (#opened: _)
   (#t: Type)
+  (p: perm)
   (a: array2 t)
   (i: U32.t)
 : SteelGhost (ith_t t) opened
-    (varray2 a)
-    (fun res -> varray2 res.ith_lhs `star` vptr res.ith_item `star` varray2 res.ith_rhs)
+    (varray2 a p)
+    (fun res -> varray2 res.ith_lhs p `star` vptrp res.ith_item p `star` varray2 res.ith_rhs p)
     (fun _ -> U32.v i < Seq.length a)
     (fun h res h' ->
       U32.v i < Seq.length a /\
       Ghost.reveal a == Seq.append res.ith_lhs (Seq.cons (Ghost.reveal res.ith_item) res.ith_rhs) /\
-      can_be_split (varray2 res.ith_lhs `star` vptr res.ith_item `star` varray2 res.ith_rhs) (varray2 res.ith_lhs) /\
-      can_be_split (varray2 res.ith_lhs `star` vptr res.ith_item `star` varray2 res.ith_rhs) (vptr res.ith_item) /\
-      can_be_split (varray2 res.ith_lhs `star` vptr res.ith_item `star` varray2 res.ith_rhs) (varray2 res.ith_lhs) /\
-      h (varray2 a) == Seq.append (h' (varray2 res.ith_lhs)) (Seq.cons (h' (vptr res.ith_item)) (h' (varray2 res.ith_rhs))) /\
+      can_be_split (varray2 res.ith_lhs p `star` vptrp res.ith_item p `star` varray2 res.ith_rhs p) (varray2 res.ith_lhs p) /\
+      can_be_split (varray2 res.ith_lhs p `star` vptrp res.ith_item p `star` varray2 res.ith_rhs p) (vptrp res.ith_item p) /\
+      can_be_split (varray2 res.ith_lhs p `star` vptrp res.ith_item p `star` varray2 res.ith_rhs p) (varray2 res.ith_lhs p) /\
+      h (varray2 a p) == Seq.append (h' (varray2 res.ith_lhs p)) (Seq.cons (h' (vptrp res.ith_item p)) (h' (varray2 res.ith_rhs p))) /\
       Seq.length res.ith_lhs == U32.v i
     )
 =
-  let m = get #(varray2 a) () in
-  let rsplit = vsplit a i in
-  reveal_star (varray2 (pfst rsplit)) (varray2 (psnd rsplit));
-  let rcons = elim_vcons (psnd rsplit) in
-  reveal_star_3 (varray2 (pfst rsplit)) (vptr (pfst rcons)) (varray2 (psnd rcons));
+  let m = get #(varray2 a p) () in
+  let rsplit = vsplit p a i in
+  reveal_star (varray2 (pfst rsplit) p) (varray2 (psnd rsplit) p);
+  let rcons = elim_vcons (psnd rsplit) p in
+  reveal_star_3 (varray2 (pfst rsplit) p) (vptrp (pfst rcons) p) (varray2 (psnd rcons) p);
   let res = { ith_lhs = pfst rsplit; ith_item = pfst rcons; ith_rhs = psnd rcons } in
   change_equal_slprop
-    (varray2 (pfst rsplit) `star` vptr (pfst rcons) `star` varray2 (psnd rcons))
-    (varray2 res.ith_lhs `star` vptr res.ith_item `star` varray2 res.ith_rhs);
-  reveal_star_3 (varray2 res.ith_lhs) (vptr res.ith_item) (varray2 res.ith_rhs);
+    (varray2 (pfst rsplit) p `star` vptrp (pfst rcons) p `star` varray2 (psnd rcons) p)
+    (varray2 res.ith_lhs p `star` vptrp res.ith_item p `star` varray2 res.ith_rhs p);
+  reveal_star_3 (varray2 res.ith_lhs p) (vptrp res.ith_item p) (varray2 res.ith_rhs p);
   res
 
 #pop-options
@@ -579,26 +600,27 @@ let unpack_ith
 let pack_ith
   (#opened: _)
   (#t: Type)
+  (p: perm)
   (res: ith_t t)
   (a: array2 t)
 : SteelGhost unit opened
-    (varray2 res.ith_lhs `star` vptr res.ith_item `star` varray2 res.ith_rhs)
-    (fun _ -> varray2 a)
+    (varray2 res.ith_lhs p `star` vptrp res.ith_item p `star` varray2 res.ith_rhs p)
+    (fun _ -> varray2 a p)
     (fun _ ->
       Ghost.reveal a == Seq.append res.ith_lhs (Seq.cons (Ghost.reveal res.ith_item) res.ith_rhs)
     )
     (fun h _ h' ->
       let i = Seq.length res.ith_lhs in
-      can_be_split (varray2 res.ith_lhs `star` vptr res.ith_item `star` varray2 res.ith_rhs) (varray2 res.ith_lhs) /\
-      can_be_split (varray2 res.ith_lhs `star` vptr res.ith_item `star` varray2 res.ith_rhs) (vptr res.ith_item) /\
-      h' (varray2 a) == Seq.append (h (varray2 res.ith_lhs)) (Seq.cons (h (vptr res.ith_item)) (h (varray2 res.ith_rhs)))
+      can_be_split (varray2 res.ith_lhs p `star` vptrp res.ith_item p `star` varray2 res.ith_rhs p) (varray2 res.ith_lhs p) /\
+      can_be_split (varray2 res.ith_lhs p `star` vptrp res.ith_item p `star` varray2 res.ith_rhs p) (vptrp res.ith_item p) /\
+      h' (varray2 a p) == Seq.append (h (varray2 res.ith_lhs p)) (Seq.cons (h (vptrp res.ith_item p)) (h (varray2 res.ith_rhs p)))
     )
 =
-  reveal_star_3 (varray2 res.ith_lhs) (vptr res.ith_item) (varray2 res.ith_rhs);
-  let rhs = intro_vcons res.ith_item res.ith_rhs in
-  reveal_star (varray2 res.ith_lhs) (varray2 rhs);
-  let a' = vappend res.ith_lhs rhs in
-  change_equal_slprop (varray2 a') (varray2 a)
+  reveal_star_3 (varray2 res.ith_lhs p) (vptrp res.ith_item p) (varray2 res.ith_rhs p);
+  let rhs = intro_vcons p res.ith_item res.ith_rhs in
+  reveal_star (varray2 res.ith_lhs p) (varray2 rhs p);
+  let a' = vappend res.ith_lhs rhs p in
+  change_equal_slprop (varray2 a' p) (varray2 a p)
 
 let seq_index_append_cons
   (#t: Type)
@@ -630,22 +652,22 @@ let rec valloc
   (x: t)
 : Steel (array1 t)
     emp
-    (fun res -> varray2 res)
+    (fun res -> varray2 res full_perm)
     (fun _ -> True)
     (fun _ res h' ->
       Seq.length res == U32.v i /\
-      h' (varray2 res) == Seq.create (U32.v i) x
+      h' (varray2 res full_perm) == Seq.create (U32.v i) x
     )
     (decreases (U32.v i))
 =
   if i = 0ul
   then
-    let res = intro_vnil t in
+    let res = intro_vnil t full_perm in
     assert (Seq.create 0 x `Seq.equal` Seq.empty);
     let res2 : array1 t = Seq.empty in
     change_equal_slprop
-      (varray2 res)
-      (varray2 res2);
+      (varray2 res full_perm)
+      (varray2 res2 full_perm);
     return res2
   else begin
     let sq : squash (i <> 0ul) = () in
@@ -656,11 +678,11 @@ let rec valloc
     change_equal_slprop
       (vptr hd)
       (vptr (Ghost.reveal (Ghost.hide hd)));
-    let res = intro_vcons (Ghost.hide hd) tl in
+    let res = intro_vcons full_perm (Ghost.hide hd) tl in
     let res2 = Seq.cons hd tl in
     change_equal_slprop
-      (varray2 res)
-      (varray2 res2);
+      (varray2 res full_perm)
+      (varray2 res2 full_perm);
     return res2
   end
 
@@ -714,15 +736,15 @@ let gsplit #t r i = tsplit r i
 
 let gsplit_unique #t r rl rr = ()
 
-val gsplit0 (#opened: _) (#t:Type) (a:array t) (i:U32.t)
+val gsplit0 (#opened: _) (#t:Type) (p: perm) (a:array t) (i:U32.t)
   : SteelGhost (Ghost.erased (array t & array t)) opened
-          (varray a)
-          (fun res -> varray (pfst res) `star` varray (psnd res))
+          (varrayp a p)
+          (fun res -> varrayp (pfst res) p `star` varrayp (psnd res) p)
           (fun _ -> U32.v i <= length a)
           (fun h res h' ->
-            let s = h (varray a) in
-            let sl = h' (varray (pfst res)) in
-            let sr = h' (varray (psnd res)) in
+            let s = h (varrayp a p) in
+            let sl = h' (varrayp (pfst res) p) in
+            let sr = h' (varrayp (psnd res) p) in
             U32.v i <= length a /\
             Ghost.reveal res == gsplit a i /\
             sl == Seq.slice s 0 (U32.v i) /\
@@ -730,67 +752,68 @@ val gsplit0 (#opened: _) (#t:Type) (a:array t) (i:U32.t)
             s == sl `Seq.append` sr
           )
 
-#push-options "--z3rlimit 16"
+#push-options "--z3rlimit 32"
 #restart-solver
-let gsplit0 #t a i =
-  let a2 = elim_varray a in
-  let res2 = vsplit a2 i in
+let gsplit0 #t p a i =
+  let a2 = elim_varray a p in
+  let res2 = vsplit p a2 i in
   let res = tsplit a i in
-  intro_varray (pfst res2) (pfst res);
-  intro_varray (psnd res2) (psnd res);
+  intro_varray p (pfst res2) (pfst res);
+  intro_varray p (psnd res2) (psnd res);
   let gres = Ghost.hide res in
   change_equal_slprop
-    (varray (pfst res))
-    (varray (pfst gres));
+    (varrayp (pfst res) p)
+    (varrayp (pfst gres) p);
   change_equal_slprop
-    (varray (psnd res))
-    (varray (psnd gres));
+    (varrayp (psnd res) p)
+    (varrayp (psnd gres) p);
   gres
 #pop-options
 
-let split #t a i =
-  let gres = gsplit0 a i in
+let splitp #t a p i =
+  let gres = gsplit0 p a i in
   let res = tsplit a i in
   change_equal_slprop
-    (varray (pfst gres))
-    (varray (pfst res));
+    (varrayp (pfst gres) p)
+    (varrayp (pfst res) p);
   change_equal_slprop
-    (varray (psnd gres))
-    (varray (psnd res));
+    (varrayp (psnd gres) p)
+    (varrayp (psnd res) p);
   return res
 
 val gjoin (#opened: _) (#t:Type) (al ar:array t)
+  (p: perm)
   : SteelGhost (Ghost.erased (array t)) opened
-          (varray al `star` varray ar)
-          (fun a -> varray a)
+          (varrayp al p `star` varrayp ar p)
+          (fun a -> varrayp a p)
           (fun _ -> adjacent al ar)
           (fun h a h' ->
-            let s = h' (varray a) in
-            s == (h (varray al) `Seq.append` h (varray ar)) /\
+            let s = h' (varrayp a p) in
+            s == (h (varrayp al p) `Seq.append` h (varrayp ar p)) /\
             merge_into al ar a
           )
 
 #push-options "--z3rlimit 32"
 #restart-solver
-let gjoin #t al ar =
-  let al2 = elim_varray al in
-  let ar2 = elim_varray ar in
-  let a2 = vappend al2 ar2 in
+let gjoin #t al ar p =
+  let al2 = elim_varray al p in
+  let ar2 = elim_varray ar p in
+  let a2 = vappend al2 ar2 p in
   let a = tmerge al ar in
-  intro_varray a2 a;
+  intro_varray p a2 a;
   let res = Ghost.hide a in
   change_equal_slprop
-    (varray a)
-    (varray (Ghost.reveal res));
+    (varrayp a p)
+    (varrayp (Ghost.reveal res) p);
   res
 #pop-options
 
-let join #t al ar =
-  let ga : Ghost.erased (array t) = gjoin al ar in
+let joinp #t al ar p =
+  let ga : Ghost.erased (array t) = gjoin al ar p in
   let a = tmerge al ar in
   change_equal_slprop
-    (varray (Ghost.reveal ga))
-    (varray a);
+    (varrayp (Ghost.reveal ga) p)
+    (varrayp a p);
   return a
 
 let freeable #t a = a.from == 0ul /\ U32.v a.to == Seq.length a.base
@@ -814,36 +837,36 @@ let alloc2 (#t:Type) (x:t) (n:U32.t)
     from = 0ul;
     to = n;
   } in
-  intro_varray (Ghost.hide base) res;
+  intro_varray full_perm (Ghost.hide base) res;
   return res
 
 let alloc x n = alloc2 x n
 
-let index #t r i =
-  let r2 = elim_varray r in
-  let p = unpack_ith r2 i in
-  let gl = gget (varray2 p.ith_lhs) in
-  let gg = gget (vptr p.ith_item) in
-  let gr = gget (varray2 p.ith_rhs) in
+let indexp #t r q i =
+  let r2 = elim_varray r q in
+  let p = unpack_ith q r2 i in
+  let gl = gget (varray2 p.ith_lhs q) in
+  let gg = gget (vptrp p.ith_item q) in
+  let gr = gget (varray2 p.ith_rhs q) in
   seq_index_append_cons (U32.v i) (Ghost.reveal gl) (Ghost.reveal gg) (Ghost.reveal gr);
   (* r2 and p are ghost,
      so the proper way is to index into base *)
   seq_index_append_cons (U32.v i) p.ith_lhs p.ith_item p.ith_rhs;
   let j : nat = U32.v r.from + U32.v i in
   let pi = Seq.index r.base j in
-  change_equal_slprop (vptr p.ith_item) (vptr pi);
-  let res = read pi in 
-  change_equal_slprop (vptr pi) (vptr p.ith_item);
-  pack_ith p r2;
-  intro_varray r2 r;
+  change_equal_slprop (vptrp p.ith_item q) (vptrp pi q);
+  let res = readp pi q in
+  change_equal_slprop (vptrp pi q) (vptrp p.ith_item q);
+  pack_ith q p r2;
+  intro_varray q r2 r;
   return res
 
 let upd #t r i x =
-  let r2 = elim_varray r in
-  let p = unpack_ith r2 i in
-  let gl = gget (varray2 p.ith_lhs) in
+  let r2 = elim_varray r _ in
+  let p = unpack_ith _ r2 i in
+  let gl = gget (varray2 p.ith_lhs _) in
   let gg = gget (vptr p.ith_item) in
-  let gr = gget (varray2 p.ith_rhs) in
+  let gr = gget (varray2 p.ith_rhs _) in
   seq_upd_append_cons (U32.v i) x (Ghost.reveal gl) (Ghost.reveal gg) (Ghost.reveal gr);
   (* r2 and p are ghost,
      so the proper way is to index into base *)
@@ -853,8 +876,8 @@ let upd #t r i x =
   change_equal_slprop (vptr p.ith_item) (vptr pi);
   write pi x;
   change_equal_slprop (vptr pi) (vptr p.ith_item);
-  pack_ith p r2;
-  intro_varray r2 r
+  pack_ith _ p r2;
+  intro_varray _ r2 r
 
 (* TODO: properly deallocate instead of just dropping the vprop *)
 let free #t r =
